Compatibility of forward simulations with linking

common/SmallstepLinking.v
@@ -1,3 +1,4 @@
+Require Import Coqlib.
 Require Import List.
 Require Import Events.
 Require Import Globalenvs.
@@ -14,23 +15,24 @@ Axiom valid_query_determ:
   forall {li} (L1 L2: open_sem li li) sk se q,
     link (skel L1) (skel L2) = Some sk -> valid_query L1 se q -> valid_query L2 se q -> False.
 
-Section LINK.
-  Context {li} (L1 L2 : Smallstep.open_sem li li).
-  Notation L i := (if i:bool then L1 else L2).
+Ltac subst_dep :=
+  subst;
+  lazymatch goal with
+    | H: existT ?P ?x _ = existT ?P ?x _ |- _ =>
+      apply inj_pair2 in H; subst_dep
+    | _ =>
+      idtac
+  end.
 
-  Ltac subst_dep :=
-    subst;
-    lazymatch goal with
-      | H: existT ?P ?x _ = existT ?P ?x _ |- _ =>
-        apply inj_pair2 in H; subst_dep
-      | _ =>
-        idtac
-    end.
+Section LINK.
+  Context {li I} (L : I -> open_sem li li).
+
+  (** * Definition *)
 
   Section WITH_SE.
     Context (se: Senv.t).
 
-    Variant frame := st (i: bool) (q: query li) (s: Smallstep.state (L i se q)).
+    Variant frame := st (i: I) (q: query li) (s: Smallstep.state (L i se q)).
     Notation state := (list frame).
 
     Inductive step: state -> trace -> state -> Prop :=
@@ -71,81 +73,91 @@ Section LINK.
 
   End WITH_SE.
 
-  Definition semantics: option (open_sem li li) :=
-    option_map
-      (fun sk =>
-        {|
-          activate se q :=
-            {|
-              Smallstep.step ge := step se;
-              Smallstep.initial_state := initial_state se q;
-              Smallstep.at_external := at_external se;
-              Smallstep.after_external := after_external se;
-              Smallstep.final_state := final_state se;
-              Smallstep.globalenv := tt;
-            |};
-          skel := sk;
-        |})
-      (link (skel L1) (skel L2)).
+  Context (sk: AST.program unit unit).
 
-  Lemma semantics_receptive L:
-    open_receptive L1 ->
-    open_receptive L2 ->
-    semantics = Some L ->
-    open_receptive L.
+  Definition semantics: open_sem li li :=
+    {|
+      activate se q :=
+        {|
+          Smallstep.step ge := step se;
+          Smallstep.initial_state := initial_state se q;
+          Smallstep.at_external := at_external se;
+          Smallstep.after_external := after_external se;
+          Smallstep.final_state := final_state se;
+          Smallstep.globalenv := tt;
+        |};
+      skel := sk;
+    |}.
+
+  (** * Properties *)
+
+  Lemma star_internal se i q s t s' k:
+    Star (L i se q) s t s' ->
+    star (fun _ => step se) tt (st se i q s :: k) t (st se i q s' :: k).
   Proof.
-    intros HL1 HL2 HL se q. unfold semantics in HL.
-    destruct link as [sk|]; inversion HL; clear HL; subst.
-    assert (forall i q, receptive (L i se q) se) by (intros [|]; auto); clear - H.
+    induction 1; [eapply star_refl | eapply star_step]; eauto.
+    constructor; auto.
+  Qed.
+
+  Lemma plus_internal se i q s t s' k:
+    Plus (L i se q) s t s' ->
+    plus (fun _ => step se) tt (st se i q s :: k) t (st se i q s' :: k).
+  Proof.
+    destruct 1; econstructor; eauto using step_internal, star_internal.
+  Qed.
+
+  (** * Receptiveness and determinacy *)
+
+  Hypothesis valid_query_excl:
+    forall i j se q, valid_query (L i) se q -> valid_query (L j) se q -> i = j.
+
+  Lemma semantics_receptive:
+    (forall i, open_receptive (L i)) ->
+    open_receptive semantics.
+  Proof.
+    intros HL se q. unfold open_receptive in HL.
     constructor; cbn.
     - intros s t1 s1 t2 STEP Ht. destruct STEP.
-      + edestruct @sr_receptive as (s2 & Hs2); eauto. 
-        eexists. eapply step_internal; eauto.
+      + edestruct @sr_receptive; eauto. eexists. eapply step_internal; eauto.
       + inversion Ht; clear Ht; subst. eexists. eapply step_push; eauto.
       + inversion Ht; clear Ht; subst. eexists. eapply step_pop; eauto.
     - intros s t s' STEP. destruct STEP; cbn; eauto.
       eapply sr_traces; eauto.
   Qed.
 
-  Lemma semantics_determinate L:
-    open_determinate L1 ->
-    open_determinate L2 ->
-    semantics = Some L ->
-    open_determinate L.
+  Lemma semantics_determinate:
+    (forall i, open_determinate (L i)) ->
+    open_determinate semantics.
   Proof.
-    intros HL1 HL2 HL se q. unfold semantics in HL.
-    destruct link as [sk|] eqn:Hsk; inversion HL; clear HL; subst.
-    assert (forall i q, determinate (L i se q) se) by (intros [|]; auto).
-    assert (forall i j q, valid_query (L i) se q -> valid_query (L j) se q -> i = j).
-    { intros. destruct i, j; eauto; eelim valid_query_determ; eauto. }
-    clear HL1 HL2. constructor; cbn.
+    intros HL se q. unfold open_determinate in HL.
+    constructor; cbn.
     - destruct 1; inversion 1; subst_dep.
-      + edestruct (sd_determ (H i q0) s t s' t2 s'0); intuition eauto; congruence.
+      + edestruct (sd_determ (HL i se q0) s t s' t2 s'0); intuition eauto; congruence.
       + eelim sd_at_external_nostep; eauto.
       + eelim sd_final_nostep; eauto.
       + eelim sd_at_external_nostep; eauto.
-      + destruct (sd_at_external_determ (H i q0) s qx qx0); eauto.
+      + destruct (sd_at_external_determ (HL i se q0) s qx qx0); eauto.
         assert (j0 = j) by eauto; subst.
-        destruct (sd_initial_determ (H j qx) s' s'0); eauto.
+        destruct (sd_initial_determ (HL j se qx) s' s'0); eauto.
         intuition auto. constructor.
       + eelim sd_final_noext; eauto.
       + eelim sd_final_nostep; eauto.
       + eelim sd_final_noext; eauto.
-      + edestruct (sd_final_determ (H i qx) s r r0); eauto.
-        edestruct (sd_after_external_determ (H j q0) sk0 r s' s'0); eauto.
+      + edestruct (sd_final_determ (HL i se qx) s r r0); eauto.
+        edestruct (sd_after_external_determ (HL j se q0) sk0 r s' s'0); eauto.
         intuition auto. constructor.
     - intros s t s' STEP. destruct STEP; cbn; eauto.
       eapply sd_traces; eauto.
     - destruct 1; inversion 1; subst. assert (i0 = i) by eauto; subst.
-      edestruct (sd_initial_determ (H i q) s s0); eauto.
+      edestruct (sd_initial_determ (HL i se q) s s0); eauto.
     - destruct 1. inversion 1; subst_dep.
       + eapply sd_at_external_nostep; eauto.
-      + edestruct (sd_at_external_determ (H i q0) s qx qx0); eauto. eapply H2; eauto.
+      + edestruct (sd_at_external_determ (HL i se q0) s qx qx0); eauto. eapply H0; eauto.
       + eapply sd_final_noext; eauto.
     - destruct 1. inversion 1; subst_dep.
       eapply sd_at_external_determ; eauto.
     - destruct 1. inversion 1; subst_dep.
-      edestruct (sd_after_external_determ (H i q0) s r s' s'0); eauto.
+      edestruct (sd_after_external_determ (HL i se q0) s r s' s'0); eauto.
     - destruct 1. inversion 1; subst_dep.
       + eapply sd_final_nostep; eauto.
       + eapply sd_final_noext; eauto.
@@ -157,11 +169,204 @@ Section LINK.
 
 End LINK.
 
-Instance Linker_open_sem li: Linker (open_sem li li) :=
+(** * Compatibility with forward simulations *)
+
+(** ** Measure *)
+
+(** Because the measure types and orders used by the simulations are
+  existentially sealed by [forward_simulation], we need to use the
+  following generic "meta-order". *)
+
+Inductive index :=
+  | mkind {T: Type} (lt: T -> T -> Prop) (Hlt: well_founded lt) (t: T).
+
+Inductive order : index -> index -> Prop :=
+  | ord_intro T (lt : T -> T -> Prop) Hlti Hltj i j:
+      lt i j -> order (mkind lt Hlti i) (mkind lt Hltj j).
+
+Lemma order_well_founded:
+  well_founded order.
+Proof.
+  clear. intros [T lt Hlt i]. pose proof (Hlt i) as Hi. revert Hlt.
+  induction Hi. constructor. intros y Hy.
+  inv Hy; subst_dep. clear - H3 H0. eauto.
+Qed.
+
+(** ** Simulation relation *)
+
+(** Likewise, we need to embed the simulation data into our simulation
+  relation. This aspect makes it a little bit convoluted but it is
+  otherwise straightforward. *)
+
+Section FSIM.
+  Context {li1 li2} (cc: callconv li1 li2).
+  Context {I L1 L2} (HL: forall i:I, open_fsim cc cc (L1 i) (L2 i)).
+  Context {sk1 sk2: AST.program unit unit}.
+  Context {w se1 se2 q1 q2}
+    (Hsk1: forall i, Senv.valid_for (skel (L1 i)) se1)
+    (Hsk: forall i, match_skel se1 se2 (skel (L1 i)) (skel (L2 i)))
+    (Hse: match_senv cc w se1 se2)
+    (Hq: match_query cc w q1 q2).
+
+  Inductive match_topframes wk: _ -> frame L1 se1 -> frame L2 se2 -> Prop :=
+    match_topframes_intro i ind ord q1 q2 s1 s2 ms idx:
+      forall (H: fsim_properties cc (match_reply cc wk) (L1 i se1 q1) (L2 i se2 q2) ind ord ms),
+      ms idx s1 s2 ->
+      match_topframes wk
+        (mkind ord (fsim_order_wf H) idx)
+        (st L1 se1 i q1 s1)
+        (st L2 se2 i q2 s2).
+
+  Inductive match_contframes wk wk': frame L1 se1 -> frame L2 se2 -> Prop :=
+    match_contframes_intro i ind ord q1 q2 s1 s2 ms:
+      forall (H: fsim_properties cc (match_reply cc wk') (L1 i se1 q1) (L2 i se2 q2) ind ord ms),
+      (forall r1 r2 s1', match_reply cc wk r1 r2 ->
+       Smallstep.after_external (L1 i se1 q1) s1 r1 s1' ->
+       exists idx s2', Smallstep.after_external (L2 i se2 q2) s2 r2 s2' /\ ms idx s1' s2') ->
+      match_contframes wk wk'
+        (st L1 se1 i q1 s1)
+        (st L2 se2 i q2 s2).
+
+  Inductive match_states: index -> list (frame L1 se1) -> list (frame L2 se2) -> Prop :=
+    | match_states_cons wk idx f1 f2 k1 k2:
+        match_topframes wk idx f1 f2 ->
+        match_cont wk k1 k2 ->
+        match_states idx (f1 :: k1) (f2 :: k2)
+  with match_cont: ccworld cc -> _ -> _ -> Prop :=
+    | match_cont_cons wk wk' f1 f2 k1 k2:
+        match_contframes wk wk' f1 f2 ->
+        match_cont wk' k1 k2 ->
+        match_cont wk (f1 :: k1) (f2 :: k2)
+    | match_cont_nil:
+        match_cont w nil nil.
+
+  (** ** Simulation properties *)
+
+  Lemma step_simulation:
+    forall idx s1 s2 t s1', match_states idx s1 s2 -> step L1 se1 s1 t s1' ->
+    exists idx' s2',
+      (plus (fun _ => step L2 se2) tt s2 t s2' \/
+       star (fun _ => step L2 se2) tt s2 t s2' /\ order idx' idx) /\
+      match_states idx' s1' s2'.
+  Proof.
+    intros idx s1 s2 t s1' Hs Hs1'.
+    destruct Hs1'; inv Hs.
+    - (* internal step *)
+      inv H3; subst_dep. clear ms H0 ms1 H8.
+      edestruct @fsim_simulation as (idx' & s2' & Hs2' & Hs'); eauto.
+      eexists (mkind ord (fsim_order_wf H6) idx'), _. split.
+      * destruct Hs2'; [left | right]; intuition eauto using star_internal, plus_internal.
+        constructor. auto.
+      * econstructor; eauto. econstructor; eauto.
+    - (* cross-component call *)
+      inv H5; subst_dep. clear ms H2 ms1 H10.
+      edestruct @fsim_match_external as (wx & qx2 & Hqx2 & Hqx & Hrx); eauto.
+      edestruct (HL j wx) as [indj ordj msj Hj]; eauto. admit. (* match_senv *)
+      edestruct @fsim_match_initial_states as (idx' & s2' & Hs2' & Hs'); eauto.
+      eexists (mkind ordj (fsim_order_wf Hj) idx'), _. split.
+      + left. apply plus_one. eapply step_push; eauto. admit. (* valid_query *)
+      + repeat (econstructor; eauto).
+    - (* cross-component return *)
+      inv H4; subst_dep. clear H1 ms H9 ms1.
+      edestruct @fsim_match_final_states as (r2 & Hr2 & Hr); eauto.
+      inv H6. inv H4; subst_dep. edestruct H9 as (idx' & s2' & Hs2'& Hs'); eauto.
+      eexists (mkind ord0 (fsim_order_wf H6) idx'), _. split.
+      + left. apply plus_one. eapply step_pop; eauto.
+      + repeat (econstructor; eauto).
+  Admitted.
+
+  Lemma initial_states_simulation:
+    forall s1, initial_state L1 se1 q1 s1 ->
+    exists idx s2, initial_state L2 se2 q2 s2 /\ match_states idx s1 s2.
+  Proof.
+    intros _ [i s1 Hq1 Hs1].
+    destruct (HL i w se1 se2 q1 q2 (Hsk1 i) (Hsk i) Hse Hq) as [ind ord ms Hms].
+    edestruct @fsim_match_initial_states as (idx & s2 & Hs2 & Hs); eauto.
+    exists (mkind ord (fsim_order_wf Hms) idx), (st L2 se2 i q2 s2 :: nil).
+    split; econstructor; eauto.
+    + admit. (* valid_query *)
+    + econstructor; eauto.
+    + constructor.
+  Admitted.
+
+  Lemma final_states_simulation:
+    forall idx s1 s2 r1, match_states idx s1 s2 -> final_state L1 se1 s1 r1 ->
+    exists r2, final_state L2 se2 s2 r2 /\ match_reply cc w r1 r2.
+  Proof.
+    clear. intros idx s1 s2 r1 Hs Hr1. destruct Hr1 as [i q1 s1 r1 Hr1].
+    inv Hs. inv H4. inv H2. subst_dep. clear ms H ms1 H6.
+    edestruct @fsim_match_final_states as (r2 & Hr2 & Hr); eauto.
+    exists r2. split; eauto. constructor; eauto.
+  Qed.
+
+  Lemma external_simulation:
+    forall idx s1 s2 qx1, match_states idx s1 s2 -> at_external L1 se1 s1 qx1 ->
+    exists wx qx2, at_external L2 se2 s2 qx2 /\ match_query cc wx qx1 qx2 /\
+    forall rx1 rx2 s1', match_reply cc wx rx1 rx2 -> after_external L1 se1 s1 rx1 s1' ->
+    exists idx' s2', after_external L2 se2 s2 rx2 s2' /\ match_states idx' s1' s2'.
+  Proof.
+    clear. intros idx s1 s2 q1 Hs Hq1. destruct Hq1 as [i q1 s1 qx1 k1 Hqx1 Hvld].
+    inv Hs. inv H2. subst_dep. clear ms H ms1 H7.
+    edestruct @fsim_match_external as (wx & qx2 & Hqx2 & Hqx & H); eauto.
+    exists wx, qx2. intuition idtac.
+    + constructor; eauto. admit. (* valid query vs. match_query *)
+    + inv H1; subst_dep.
+      edestruct H as (idx' & s2' & Hs2' & Hs'); eauto.
+      eexists (mkind _ (fsim_order_wf H5) idx'), _.
+      split; repeat (econstructor; eauto).
+  Admitted.
+
+  Lemma semantics_simulation:
+    fsim_properties cc (match_reply cc w)
+      (semantics L1 sk1 se1 q1)
+      (semantics L2 sk2 se2 q2)
+      index order match_states.
+  Proof.
+    split; cbn.
+    - apply order_well_founded.
+    - eauto using initial_states_simulation.
+    - eauto using final_states_simulation.
+    - eauto using external_simulation.
+    - eauto using step_simulation.
+  Qed.
+
+End FSIM.
+
+(** * Linking operator *)
+
+Local Unset Program Cases.
+
+Program Instance Linker_open_sem li: Linker (open_sem li li) :=
   {
-    link L1 L2 := semantics L1 L2;
-    linkorder := open_fsim cc_id cc_id;
+    link La Lb :=
+      let L i := match i with true => La | false => Lb end in
+      option_map (semantics L) (link (skel La) (skel Lb));
+    linkorder :=
+      open_fsim cc_id cc_id;
   }.
-(* Need to prove: identity and composition for fsim,
-  fsim between component and linked program. *)    
+Next Obligation.
+  (* identity simulation *)
+Admitted.
+Next Obligation.
+  (* vertical composition of simulations *)
+Admitted.
+Next Obligation.
+  (* fsim between component and linked program (?) *)
+Admitted.
+
+Lemma link_simulation {li1 li2} (cc: callconv li1 li2) L1a L1b L1 L2a L2b L2:
+  open_fsim cc cc L1a L2a ->
+  open_fsim cc cc L1b L2b ->
+  link L1a L1b = Some L1 ->
+  link L2a L2b = Some L2 ->
+  open_fsim cc cc L1 L2.
+Proof.
+  intros Ha Hb H1 H2. cbn in *. unfold option_map in *.
+  destruct (link (skel L1a) (skel L1b)) as [sk1|] eqn:Hsk1; try discriminate. inv H1.
+  destruct (link (skel L2a) (skel L2b)) as [sk2|] eqn:Hsk2; try discriminate. inv H2.
+  intros w se1 se2 q1 q2. simpl. intros Hse1 Hsk Hse Hq.
+  econstructor. eapply semantics_simulation; eauto.
+  - intros [|]; auto.
+  - admit. (* Senv.valid_for vs. skeleton linking *)
+  - admit. (* match_skel vs. skeleton linking *)
 Admitted.
